\documentclass{article}

\usepackage{amssymb}


\begin{document}

\section{Question 1}
\subsection{a}
\[\vec{\nabla} \cdot (\vec{\nabla} \times \vec{V}) = \partial_l (\eta^{li}\epsilon_{ijk}\partial^jV^k)\]
\[=\partial^i\epsilon_{ijk}\partial^jV^k=\epsilon_{ijk}\partial^i\partial^jV^k\]
\[=\frac{1}{2}(\epsilon_{ijk}\partial^i\partial^jV^k + \epsilon_{jik}\partial^j\partial^iV^k)\]
\[=\frac{1}{2}(\epsilon_{ijk}\partial^i\partial^jV^k - \epsilon_{ijk}\partial^j\partial^iV^k)\]
\[=\frac{1}{2}(\epsilon_{ijk}\partial^i\partial^jV^k - \epsilon_{ijk}\partial^i\partial^jV^k) = 0 \hspace{1em} \square \]



\end{document}